coq/theories/assembly/ASMSemantics.v
@@ -5,6 +5,7 @@ Require Import impboot.assembly.ASMSyntax.
 Require Import coqutil.Word.Interface.
 Require Import coqutil.Word.Properties.
 From Stdlib Require Import Relations.Relation_Operators.
+From Stdlib Require Import Program.Equality.
 
 Inductive word_or_ret :=
 | Word : word64 -> word_or_ret
@@ -245,11 +246,21 @@ Inductive steps : (s_or_h * nat) -> (s_or_h * nat) -> Prop :=
   steps (s2, n2) (s3, n3) ->
   steps (s1, n1) (s3, n3).
 
-(* TODO(kπ) something like this *)
-(* Lemma steps_add_fuel: forall s1 n1 s2 n2 s3 n3,
-  steps (s1, n1) (s2, 0) ->
-  steps (s2, n2) (s3, n3) ->
-  steps (s1, n1 + n2) (s3, n3) *)
+Lemma steps_add_fuel: forall s1 n1 s2 n2 x,
+  steps (s1, n1) (s2, n2) ->
+  steps (s1, n1 + x) (s2, n2 + x).
+Proof.
+  intros.
+  dependent induction H.
+  - simpl. eapply steps_refl.
+  - eapply steps_step_same.
+    eauto.
+  - replace (n2 + 1 + x) with (n2 + x + 1) by lia.
+    simpl.
+    eapply steps_step_succ.
+    eauto.
+  - eapply steps_trans; eauto.
+Qed.
 
 Definition can_write_mem_at (m : word64 -> option (option word64)) (a : word64) : Prop :=
   m a = Some None.
